theories/zoo_saturn/inf_ws_deque_2.v
@@ -1,7 +1,10 @@
 From zoo Require Import
   prelude.
 From zoo.common Require Import
-  list.
+  countable
+  relations.
+From zoo.iris.base_logic Require Import
+  lib.auth_twins.
 From zoo.language Require Import
   notations.
 From zoo.iris.bi Require Import
@@ -18,57 +21,517 @@ From zoo_saturn Require Import
 From zoo Require Import
   options.
 
-Implicit Types v t : val.
+Import inf_ws_deque_1.base.
 
-Class InfWsQueue2G Σ `{zoo_G : !ZooG Σ} := {
-  #[local] inf_ws_deque_2_G :: InfWsQueue1G Σ ;
+Implicit Types slot : location.
+Implicit Types slots : list location.
+Implicit Types v : val.
+Implicit Types vs ws : list val.
+
+Class InfWsDeque2G Σ `{zoo_G : !ZooG Σ} := {
+  #[local] inf_ws_deque_2_G_base_G :: InfWsDeque1G Σ ;
+  #[local] inf_ws_deque_2_G_model_G :: AuthTwinsG Σ (leibnizO (list val)) suffix ;
 }.
 
 Definition inf_ws_deque_2_Σ := #[
-  inf_ws_deque_1_Σ
+  inf_ws_deque_1_Σ ;
+  auth_twins_Σ (leibnizO (list val)) suffix
 ].
 #[global] Instance subG_inf_ws_deque_2_Σ Σ `{zoo_G : !ZooG Σ} :
   subG inf_ws_deque_2_Σ Σ →
-  InfWsQueue2G Σ .
+  InfWsDeque2G Σ .
 Proof.
   solve_inG.
 Qed.
 
-Section inf_ws_deque_2_G.
-  Context `{inf_ws_deque_2_G : InfWsQueue2G Σ}.
+Module base.
+  Section inf_ws_deque_2_G.
+    Context `{inf_ws_deque_2_G : InfWsDeque2G Σ}.
 
-  Definition inf_ws_deque_2_inv :=
-    inf_ws_deque_1_inv.
+    Implicit Types t : location.
+
+    Record inf_ws_deque_2_name := {
+      inf_ws_deque_2_name_base : inf_ws_deque_1_name ;
+      inf_ws_deque_2_name_model : auth_twins_name ;
+    }.
+    Implicit Type γ : inf_ws_deque_2_name.
+
+    #[global] Instance inf_ws_deque_2_name_eq_dec : EqDecision inf_ws_deque_2_name :=
+      ltac:(solve_decision).
+    #[global] Instance inf_ws_deque_2_name_countable :
+      Countable inf_ws_deque_2_name.
+    Proof.
+      solve_countable.
+    Qed.
+
+    #[local] Definition model₁' γ_model vs :=
+      auth_twins_twin1 _ γ_model vs.
+    #[local] Definition model₁ γ :=
+      model₁' γ.(inf_ws_deque_2_name_model).
+    #[local] Definition model₂' γ_model vs :=
+      auth_twins_twin2 _ γ_model vs.
+    #[local] Definition model₂ γ :=
+      model₂' γ.(inf_ws_deque_2_name_model).
+
+    #[local] Definition owner' γ_owner ws :=
+      auth_twins_auth _ γ_owner ws.
+    #[local] Definition owner γ :=
+      owner' γ.(inf_ws_deque_2_name_model).
+
+    #[local] Definition inv_inner γ : iProp Σ :=
+      ∃ vs slots,
+      inf_ws_deque_1_model γ.(inf_ws_deque_2_name_base) (#@{location} <$> slots) ∗
+      model₂ γ vs ∗
+      [∗ list] slot; v ∈ slots; vs, slot ↦ᵣ v.
+    #[local] Instance : CustomIpat "inv_inner" :=
+      " ( %vs{} &
+          %slots{} &
+          >Hbase_model &
+          >Hmodel₂ &
+          >Hslots
+        )
+      ".
+    Definition inf_ws_deque_2_inv t γ ι : iProp Σ :=
+      inf_ws_deque_1_inv t γ.(inf_ws_deque_2_name_base) (ι.@"base") ∗
+      inv (ι.@"inv") (inv_inner γ).
+    #[local] Instance : CustomIpat "inv" :=
+      " ( #Hbase_inv &
+          #Hinv
+        )
+      ".
+
+    Definition inf_ws_deque_2_model :=
+      model₁.
+    #[local] Instance : CustomIpat "model" :=
+      " Hmodel₁{_{}}
+      ".
+
+    Definition inf_ws_deque_2_owner γ ws : iProp Σ :=
+      ∃ slots_owner,
+      inf_ws_deque_1_owner γ.(inf_ws_deque_2_name_base) (#@{location} <$> slots_owner) ∗
+      owner γ ws.
+    #[local] Instance : CustomIpat "owner" :=
+      " ( %slots_owner{_{}} &
+          Hbase_owner{_{}} &
+          Howner{_{}}
+        )
+      ".
+
+    #[global] Instance inf_ws_deque_2_model_timeless γ vs :
+      Timeless (inf_ws_deque_2_model γ vs).
+    Proof.
+      apply _.
+    Qed.
+    #[global] Instance inf_ws_deque_2_owner_timeless γ ws :
+      Timeless (inf_ws_deque_2_owner γ ws).
+    Proof.
+      apply _.
+    Qed.
+
+    #[global] Instance inf_ws_deque_2_inv_persistent t γ ι :
+      Persistent (inf_ws_deque_2_inv t γ ι).
+    Proof.
+      apply _.
+    Qed.
+
+    #[local] Lemma model_owner_alloc :
+      ⊢ |==>
+        ∃ γ_model,
+        model₁' γ_model [] ∗
+        model₂' γ_model [] ∗
+        owner' γ_model [].
+    Proof.
+      iMod (auth_twins_alloc (auth_twins_G := inf_ws_deque_2_G_model_G) _ []) as "(%γ_model & $ & $ & $)".
+      iSteps.
+    Qed.
+    #[local] Lemma model₁_valid γ ws vs :
+      owner γ ws -∗
+      model₁ γ vs -∗
+      ⌜vs `suffix_of` ws⌝.
+    Proof.
+      rewrite -preorder_rtc.
+      apply: auth_twins_valid_1.
+    Qed.
+    #[local] Lemma model₁_exclusive γ vs1 vs2 :
+      model₁ γ vs1 -∗
+      model₁ γ vs2 -∗
+      False.
+    Proof.
+      apply auth_twins_twin1_exclusive.
+    Qed.
+    #[local] Lemma model₂_valid γ ws vs :
+      owner γ ws -∗
+      model₂ γ vs -∗
+      ⌜vs `suffix_of` ws⌝.
+    Proof.
+      rewrite -preorder_rtc.
+      apply: auth_twins_valid_2.
+    Qed.
+    #[local] Lemma model_agree γ vs1 vs2 :
+      model₁ γ vs1 -∗
+      model₂ γ vs2 -∗
+      ⌜vs1 = vs2⌝.
+    Proof.
+      apply: auth_twins_agree_L.
+    Qed.
+    #[local] Lemma model_owner_agree γ ws vs1 vs2 :
+      owner γ ws -∗
+      model₁ γ vs1 -∗
+      model₂ γ vs2 -∗
+        ⌜vs1 `suffix_of` ws⌝ ∗
+        ⌜vs1 = vs2⌝.
+    Proof.
+      iIntros "Howner₁ Hmodel₁ Hmodel₂".
+      iDestruct (model₁_valid with "Howner₁ Hmodel₁") as %Hsuffix.
+      iDestruct (model_agree with "Hmodel₁ Hmodel₂") as %->.
+      iSteps.
+    Qed.
+    #[local] Lemma model_empty {γ ws vs1 vs2} :
+      owner γ ws -∗
+      model₁ γ vs1 -∗
+      model₂ γ vs2 ==∗
+        owner γ [] ∗
+        model₁ γ [] ∗
+        model₂ γ [].
+    Proof.
+      apply auth_twins_update_auth.
+    Qed.
+    #[local] Lemma model_push {γ ws vs1 vs2} v :
+      owner γ ws -∗
+      model₁ γ vs1 -∗
+      model₂ γ vs2 ==∗
+        owner γ (vs1 ++ [v]) ∗
+        model₁ γ (vs1 ++ [v]) ∗
+        model₂ γ (vs1 ++ [v]).
+    Proof.
+      apply auth_twins_update_auth.
+    Qed.
+    #[local] Lemma model_steal γ vs1 vs2 :
+      model₁ γ vs1 -∗
+      model₂ γ vs2 ==∗
+        model₁ γ (tail vs1) ∗
+        model₂ γ (tail vs1).
+    Proof.
+      apply: auth_twins_update_twins_L.
+      rewrite preorder_rtc. apply suffix_tail. done.
+    Qed.
+    #[local] Lemma model_pop γ ws vs1 vs2 :
+      owner γ ws -∗
+      model₁ γ vs1 -∗
+      model₂ γ vs2 ==∗
+        owner γ (removelast vs1) ∗
+        model₁ γ (removelast vs1) ∗
+        model₂ γ (removelast vs1).
+    Proof.
+      apply auth_twins_update_auth.
+    Qed.
+
+    #[local] Lemma owner_update γ ws vs :
+      owner γ ws -∗
+      model₁ γ vs -∗
+      model₂ γ vs ==∗
+        owner γ vs ∗
+        model₁ γ vs ∗
+        model₂ γ vs.
+    Proof.
+      apply auth_twins_update_auth.
+    Qed.
+    #[local] Lemma owner_exclusive γ ws1 ws2 :
+      owner γ ws1 -∗
+      owner γ ws2 -∗
+      False.
+    Proof.
+      apply: auth_twins_auth_exclusive.
+    Qed.
+
+    Lemma inf_ws_deque_2_model_exclusive γ vs1 vs2 :
+      inf_ws_deque_2_model γ vs1 -∗
+      inf_ws_deque_2_model γ vs2 -∗
+      False.
+    Proof.
+      iIntros "(:model =1) (:model =2)".
+      iApply (model₁_exclusive with "Hmodel₁_1 Hmodel₁_2").
+    Qed.
+
+    Lemma inf_ws_deque_2_owner_exclusive γ ws1 ws2 :
+      inf_ws_deque_2_owner γ ws1 -∗
+      inf_ws_deque_2_owner γ ws2 -∗
+      False.
+    Proof.
+      iIntros "(:owner =1) (:owner =2)".
+      iApply (owner_exclusive with "Howner_1 Howner_2").
+    Qed.
+    Lemma inf_ws_deque_2_owner_model γ ws vs :
+      inf_ws_deque_2_owner γ ws -∗
+      inf_ws_deque_2_model γ vs -∗
+      ⌜vs `suffix_of` ws⌝.
+    Proof.
+      iIntros "(:owner =1) (:model =2)".
+      iApply (model₁_valid with "Howner_1 Hmodel₁_2").
+    Qed.
+
+    Lemma inf_ws_deque_2_create_spec ι :
+      {{{
+        True
+      }}}
+        inf_ws_deque_2_create ()
+      {{{ t γ,
+        RET #t;
+        meta_token t ⊤ ∗
+        inf_ws_deque_2_inv t γ ι ∗
+        inf_ws_deque_2_model γ [] ∗
+        inf_ws_deque_2_owner γ []
+      }}}.
+    Proof.
+      iIntros "%Φ _ HΦ".
+
+      iApply wp_fupd.
+      wp_apply (inf_ws_deque_1_create_spec with "[//]") as (t γ_base) "(Hmeta & #Hbase_inv & Hbase_model & Hbase_owner)".
+
+      iMod model_owner_alloc as "(%γ_model & Hmodel₁ & Hmodel₂ & Howner)".
+
+      pose γ := {|
+        inf_ws_deque_2_name_base := γ_base ;
+        inf_ws_deque_2_name_model := γ_model ;
+      |}.
+
+      iApply ("HΦ" $! t γ).
+      iFrame "#∗". iSplitR "Hbase_owner".
+      - iApply inv_alloc.
+        iExists [], []. iFrameSteps.
+      - iExists []. iFrameSteps.
+    Qed.
+
+    Lemma inf_ws_deque_2_size_spec t γ ι ws :
+      <<<
+        inf_ws_deque_2_inv t γ ι ∗
+        inf_ws_deque_2_owner γ ws
+      | ∀∀ vs,
+        inf_ws_deque_2_model γ vs
+      >>>
+        inf_ws_deque_2_size #t @ ↑ι
+      <<<
+        ⌜vs `suffix_of` ws⌝ ∗
+        inf_ws_deque_2_model γ vs
+      | RET #(length vs);
+        inf_ws_deque_2_owner γ vs
+      >>>.
+    Proof.
+      iIntros "%Φ ((:inv) & (:owner)) HΦ".
+
+      awp_apply (inf_ws_deque_1_size_spec with "[$]").
+      iInv "Hinv" as "(:inv_inner)".
+      iApply (aacc_aupd_commit with "HΦ"). 1: solve_ndisj. iIntros "%vs_ (:model)".
+      iAaccIntro with "Hbase_model". 1: iSteps.
+      iDestruct (model_owner_agree with "Howner Hmodel₁ Hmodel₂") as %(Hsuffix & ->).
+      iMod (owner_update with "Howner Hmodel₁ Hmodel₂") as "(Howner & $ & Hmodel₂)".
+      rewrite length_fmap.
+      iDestruct (big_sepL2_length with "Hslots") as %->.
+      iSteps.
+    Qed.
+
+    Lemma inf_ws_deque_2_is_empty_spec t γ ι ws :
+      <<<
+        inf_ws_deque_2_inv t γ ι ∗
+        inf_ws_deque_2_owner γ ws
+      | ∀∀ vs,
+        inf_ws_deque_2_model γ vs
+      >>>
+        inf_ws_deque_2_is_empty #t @ ↑ι
+      <<<
+        ⌜vs `suffix_of` ws⌝ ∗
+        inf_ws_deque_2_model γ vs
+      | RET #(bool_decide (vs = []%list));
+        inf_ws_deque_2_owner γ vs
+      >>>.
+    Proof.
+      iIntros "%Φ ((:inv) & (:owner)) HΦ".
+
+      awp_apply (inf_ws_deque_1_is_empty_spec with "[$]").
+      iInv "Hinv" as "(:inv_inner)".
+      iApply (aacc_aupd_commit with "HΦ"). 1: solve_ndisj. iIntros "%vs_ (:model)".
+      iAaccIntro with "Hbase_model". 1: iSteps.
+      iDestruct (model_owner_agree with "Howner Hmodel₁ Hmodel₂") as %(Hsuffix & ->).
+      iMod (owner_update with "Howner Hmodel₁ Hmodel₂") as "(Howner & $ & Hmodel₂)".
+      erewrite (bool_decide_ext (_ <$> _ = []) (length _ = 0)). 2: rewrite length_zero_iff_nil //.
+      rewrite length_fmap.
+      iDestruct (big_sepL2_length with "Hslots") as %->.
+      erewrite (bool_decide_ext (length _ = 0)). 2: apply length_zero_iff_nil.
+      iSteps.
+    Qed.
+
+    Lemma inf_ws_deque_2_push_spec t γ ι ws v :
+      <<<
+        inf_ws_deque_2_inv t γ ι ∗
+        inf_ws_deque_2_owner γ ws
+      | ∀∀ vs,
+        inf_ws_deque_2_model γ vs
+      >>>
+        inf_ws_deque_2_push #t v @ ↑ι
+      <<<
+        ⌜vs `suffix_of` ws⌝ ∗
+        inf_ws_deque_2_model γ (vs ++ [v])
+      | RET ();
+        inf_ws_deque_2_owner γ (vs ++ [v])
+      >>>.
+    Proof.
+      iIntros "%Φ ((:inv) & (:owner)) HΦ".
+
+      wp_rec.
+      wp_ref slot as "Hslot".
+
+      awp_apply (inf_ws_deque_1_push_spec with "[$]").
+      iInv "Hinv" as "(:inv_inner)".
+      iApply (aacc_aupd_commit with "HΦ"). 1: solve_ndisj. iIntros "%vs_ (:model)".
+      iAaccIntro with "Hbase_model". 1: iSteps.
+      iDestruct (model_owner_agree with "Howner Hmodel₁ Hmodel₂") as %(Hsuffix & ->).
+      iMod (model_push with "Howner Hmodel₁ Hmodel₂") as "(Howner & $ & Hmodel₂)".
+      iDestruct (big_sepL2_snoc_2 with "Hslots Hslot") as "Hslots".
+      rewrite -fmap_snoc. iSteps.
+    Qed.
+
+    Lemma inf_ws_deque_2_steal_spec t γ ι :
+      <<<
+        inf_ws_deque_2_inv t γ ι
+      | ∀∀ vs,
+        inf_ws_deque_2_model γ vs
+      >>>
+        inf_ws_deque_2_steal #t @ ↑ι
+      <<<
+        inf_ws_deque_2_model γ (tail vs)
+      | RET head vs;
+        True
+      >>>.
+    Proof.
+      iIntros "%Φ (:inv) HΦ".
+
+      wp_rec.
+
+      awp_apply (inf_ws_deque_1_steal_spec with "[$]").
+      iInv "Hinv" as "(:inv_inner)".
+      iApply (aacc_aupd_commit with "HΦ"). 1: solve_ndisj. iIntros "%vs_ (:model)".
+      iAaccIntro with "Hbase_model". 1: iSteps. iIntros "Hbase_model".
+      iDestruct (model_agree with "Hmodel₁ Hmodel₂") as %->.
+      iMod (model_steal with "Hmodel₁ Hmodel₂") as "($ & Hmodel₂)".
+      iIntros "!> HΦ !>".
+      destruct slots as [| slot slots], vs as [| v vs] => //.
+      all: iFrameSteps.
+    Qed.
+
+    Lemma inf_ws_deque_2_pop_spec t γ ι ws :
+      <<<
+        inf_ws_deque_2_inv t γ ι ∗
+        inf_ws_deque_2_owner γ ws
+      | ∀∀ vs,
+        inf_ws_deque_2_model γ vs
+      >>>
+        inf_ws_deque_2_pop #t @ ↑ι
+      <<<
+        ∃∃ o ws',
+        ⌜vs `suffix_of` ws⌝ ∗
+        match o with
+        | None =>
+            ⌜vs = []⌝ ∗
+            ⌜ws' = []⌝ ∗
+            inf_ws_deque_2_model γ []
+        | Some v =>
+            ∃ vs',
+            ⌜vs = vs' ++ [v]⌝ ∗
+            ⌜ws' = vs'⌝ ∗
+            inf_ws_deque_2_model γ vs'
+        end
+      | RET o;
+        inf_ws_deque_2_owner γ ws'
+      >>>.
+    Proof.
+      iIntros "%Φ ((:inv) & (:owner)) HΦ".
+
+      wp_rec.
+
+      awp_smart_apply (inf_ws_deque_1_pop_spec with "[$]").
+      iInv "Hinv" as "(:inv_inner)".
+      iApply (aacc_aupd_commit with "HΦ"). 1: solve_ndisj. iIntros "%vs_ (:model)".
+      iAaccIntro with "Hbase_model". 1: iSteps. iIntros "%o %𝑠𝑙𝑜𝑡s_owner (_ & Ho)".
+      iDestruct (model_owner_agree with "Howner Hmodel₁ Hmodel₂") as %(Hsuffix & ->).
+      iMod (model_pop with "Howner Hmodel₁ Hmodel₂") as "(Howner & Hmodel₁ & Hmodel₂)".
+      destruct o as [𝑠𝑙𝑜𝑡 |].
+
+      - iDestruct "Ho" as "(%𝑠𝑙𝑜𝑡s' & %Hslots & -> & Hbase_model)".
+        apply fmap_snoc_inv in Hslots as (slots' & slot & -> & -> & ->).
+        iDestruct (big_sepL2_snoc_inv_l with "Hslots") as "(%vs' & %v & -> & Hslots & Hslot)".
+        rewrite removelast_last.
+        iExists (Some v), vs'. iFrameSteps.
+
+      - iDestruct "Ho" as "(%Hslots & -> & Hbase_model)".
+        apply fmap_nil_inv in Hslots as ->.
+        iDestruct (big_sepL2_nil_inv_l with "Hslots") as %->.
+        iExists None. iFrameSteps. do 2 (iExists []; iSteps).
+    Qed.
+  End inf_ws_deque_2_G.
+
+  #[global] Opaque inf_ws_deque_2_inv.
+  #[global] Opaque inf_ws_deque_2_model.
+  #[global] Opaque inf_ws_deque_2_owner.
+End base.
+
+From zoo_saturn Require
+  inf_ws_deque_2__opaque.
+
+Section inf_ws_deque_2_G.
+  Context `{inf_ws_deque_2_G : InfWsDeque2G Σ}.
+
+  Implicit Types 𝑡 : location.
+  Implicit Types t : val.
+
+  Definition inf_ws_deque_2_inv t ι : iProp Σ :=
+    ∃ 𝑡 γ,
+    ⌜t = #𝑡⌝ ∗
+    meta 𝑡 nroot γ ∗
+    base.inf_ws_deque_2_inv 𝑡 γ ι.
+  #[local] Instance : CustomIpat "inv" :=
+    " ( %𝑡{} &
+        %γ{} &
+        {%Heq{};->} &
+        #Hmeta{_{}} &
+        Hinv{_{}}
+      )
+    ".
 
   Definition inf_ws_deque_2_model t vs : iProp Σ :=
-    ∃ slots,
-    inf_ws_deque_1_model t (#@{location} <$> slots) ∗
-    [∗ list] slot; v ∈ slots; vs, slot ↦ᵣ□ v.
+    ∃ 𝑡 γ,
+    ⌜t = #𝑡⌝ ∗
+    meta 𝑡 nroot γ ∗
+    base.inf_ws_deque_2_model γ vs.
   #[local] Instance : CustomIpat "model" :=
-    " ( %slots_vs{} &
-        Hmodel{_{}} &
-        #Hslots_vs{}
+    " ( %𝑡{} &
+        %γ{} &
+        {%Heq{};->} &
+        #Hmeta{_{}} &
+        Hmodel{_{}}
       )
     ".
 
   Definition inf_ws_deque_2_owner t ws : iProp Σ :=
-    ∃ slots,
-    inf_ws_deque_1_owner t (#@{location} <$> slots) ∗
-    [∗ list] slot; v ∈ slots; ws, slot ↦ᵣ□ v.
+    ∃ 𝑡 γ,
+    ⌜t = #𝑡⌝ ∗
+    meta 𝑡 nroot γ ∗
+    base.inf_ws_deque_2_owner γ ws.
   #[local] Instance : CustomIpat "owner" :=
-    " ( %slots_ws{} &
-        Howner{_{}} &
-        #Hslots_ws{}
+    " ( %𝑡{} &
+        %γ{} &
+        {%Heq{};->} &
+        #Hmeta{_{}} &
+        Howner{_{}}
       )
     ".
 
-  #[global] Instance inf_ws_deque_2_model_timeless t vs :
-    Timeless (inf_ws_deque_2_model t vs).
+  #[global] Instance inf_ws_deque_2_model_timeless γ vs :
+    Timeless (inf_ws_deque_2_model γ vs).
   Proof.
     apply _.
   Qed.
-  #[global] Instance inf_ws_deque_2_owner_timeless t ws :
-    Timeless (inf_ws_deque_2_owner t ws).
+  #[global] Instance inf_ws_deque_2_owner_timeless γ ws :
+    Timeless (inf_ws_deque_2_owner γ ws).
   Proof.
     apply _.
   Qed.
@@ -84,8 +547,9 @@ Section inf_ws_deque_2_G.
     inf_ws_deque_2_model t vs2 -∗
     False.
   Proof.
-    iIntros "(:model =1) (:model =2)".
-    iApply (inf_ws_deque_1_model_exclusive with "Hmodel_1 Hmodel_2").
+    iIntros "(:model =1) (:model =2)". simplify.
+    iDestruct (meta_agree with "Hmeta_1 Hmeta_2") as %->.
+    iApply (base.inf_ws_deque_2_model_exclusive with "Hmodel_1 Hmodel_2").
   Qed.
 
   Lemma inf_ws_deque_2_owner_exclusive t ws1 ws2 :
@@ -93,19 +557,18 @@ Section inf_ws_deque_2_G.
     inf_ws_deque_2_owner t ws2 -∗
     False.
   Proof.
-    iIntros "(:owner =1) (:owner =2)".
-    iApply (inf_ws_deque_1_owner_exclusive with "Howner_1 Howner_2").
+    iIntros "(:owner =1) (:owner =2)". simplify.
+    iDestruct (meta_agree with "Hmeta_1 Hmeta_2") as %->.
+    iApply (base.inf_ws_deque_2_owner_exclusive with "Howner_1 Howner_2").
   Qed.
-  Lemma inf_ws_deque_2_owner_model t ws vs :
-    inf_ws_deque_2_owner t ws -∗
-    inf_ws_deque_2_model t vs -∗
+  Lemma inf_ws_deque_2_owner_model γ ws vs :
+    inf_ws_deque_2_owner γ ws -∗
+    inf_ws_deque_2_model γ vs -∗
     ⌜vs `suffix_of` ws⌝.
   Proof.
-    iIntros "(:owner =1) (:model)".
-    iDestruct (inf_ws_deque_1_owner_model with "Howner_1 Hmodel") as %(slots & ->)%suffix_fmap; last congruence.
-    iDestruct (big_sepL2_app_inv_l with "Hslots_ws1") as "(%ws1 & %vs_ & -> & _ & Hslots_vs_)".
-    iDestruct (big_sepL2_ref_pointsto_agree with "Hslots_vs Hslots_vs_") as %<-.
-    iExists ws1. iSteps.
+    iIntros "(:owner =1) (:model =2)". simplify.
+    iDestruct (meta_agree with "Hmeta_1 Hmeta_2") as %->.
+    iApply (base.inf_ws_deque_2_owner_model with "Howner_1 Hmodel_2").
   Qed.
 
   Lemma inf_ws_deque_2_create_spec ι :
@@ -122,9 +585,10 @@ Section inf_ws_deque_2_G.
   Proof.
     iIntros "%Φ _ HΦ".
 
-    wp_apply (inf_ws_deque_1_create_spec with "[//]") as (t) "(#Hinv & Hmodel & Howner)".
-
-    iSteps. iExists []. iSteps. iExists []. iSteps.
+    iApply wp_fupd.
+    wp_apply (base.inf_ws_deque_2_create_spec with "[//]") as (𝑡 γ) "(Hmeta & Hinv & Hmodel)".
+    iMod (meta_set γ with "Hmeta"); first done.
+    iSteps.
   Qed.
 
   Lemma inf_ws_deque_2_size_spec t ι ws :
@@ -142,17 +606,14 @@ Section inf_ws_deque_2_G.
       inf_ws_deque_2_owner t vs
     >>>.
   Proof.
-    iIntros "%Φ (#Hinv & (:owner)) HΦ".
+    iIntros "%Φ ((:inv =1) & (:owner =2)) HΦ". simplify.
+    iDestruct (meta_agree with "Hmeta_1 Hmeta_2") as %->. iClear "Hmeta_1".
 
-    awp_apply (inf_ws_deque_1_size_spec with "[$]") without "Hslots_ws".
-    iApply (aacc_aupd_commit with "HΦ"); first done. iIntros "%vs (:model)".
-    iAaccIntro with "Hmodel"; first iSteps.
-    iSteps --silent / as (Hsuffix%suffix_fmap) / as (_) "HΦ Howner".
-    { iApply (big_sepL2_ref_pointsto_suffix with "Hslots_vs Hslots_ws"); first done. }
-    { congruence. }
-    rewrite length_fmap.
-    iDestruct (big_sepL2_length with "Hslots_vs") as %->.
-    iSteps.
+    awp_apply (base.inf_ws_deque_2_size_spec with "[$]").
+    { iApply (aacc_aupd_commit with "HΦ"); first done. iIntros "%vs (:model =1)". simplify.
+      iDestruct (meta_agree with "Hmeta_1 Hmeta_2") as %<-. iClear "Hmeta_2".
+      iAaccIntro with "Hmodel_1"; iSteps.
+    }
   Qed.
 
   Lemma inf_ws_deque_2_is_empty_spec t ι ws :
@@ -170,19 +631,14 @@ Section inf_ws_deque_2_G.
       inf_ws_deque_2_owner t vs
     >>>.
   Proof.
-    iIntros "%Φ (#Hinv & (:owner)) HΦ".
+    iIntros "%Φ ((:inv =1) & (:owner =2)) HΦ". simplify.
+    iDestruct (meta_agree with "Hmeta_1 Hmeta_2") as %->. iClear "Hmeta_1".
 
-    awp_apply (inf_ws_deque_1_is_empty_spec with "[$]") without "Hslots_ws".
-    iApply (aacc_aupd_commit with "HΦ"); first done. iIntros "%vs (:model)".
-    iAaccIntro with "Hmodel"; first iSteps.
-    iSteps --silent / as (Hsuffix%suffix_fmap) / as (_) "HΦ Howner".
-    { iApply (big_sepL2_ref_pointsto_suffix with "Hslots_vs Hslots_ws"); first done. }
-    { congruence. }
-    erewrite (bool_decide_ext (_ <$> _ = []) (length _ = 0)); last rewrite length_zero_iff_nil //.
-    rewrite length_fmap.
-    iDestruct (big_sepL2_length with "Hslots_vs") as %->.
-    erewrite (bool_decide_ext (length _ = 0)); last apply length_zero_iff_nil.
-    iSteps.
+    awp_apply (base.inf_ws_deque_2_is_empty_spec with "[$]").
+    { iApply (aacc_aupd_commit with "HΦ"); first done. iIntros "%vs (:model =1)". simplify.
+      iDestruct (meta_agree with "Hmeta_1 Hmeta_2") as %<-. iClear "Hmeta_2".
+      iAaccIntro with "Hmodel_1"; iSteps.
+    }
   Qed.
 
   Lemma inf_ws_deque_2_push_spec t ι ws v :
@@ -200,19 +656,14 @@ Section inf_ws_deque_2_G.
       inf_ws_deque_2_owner t (vs ++ [v])
     >>>.
   Proof.
-    iIntros "%Φ (#Hinv & (:owner)) HΦ".
+    iIntros "%Φ ((:inv =1) & (:owner =2)) HΦ". simplify.
+    iDestruct (meta_agree with "Hmeta_1 Hmeta_2") as %->. iClear "Hmeta_1".
 
-    wp_rec.
-    wp_ref slot as "Hslot".
-    iMod (pointsto_persist with "Hslot") as "Hslot".
-
-    awp_apply (inf_ws_deque_1_push_spec with "[$Hinv $Howner]").
-    iApply (aacc_aupd_commit with "HΦ"); first done. iIntros "%vs (:model)".
-    iAaccIntro with "Hmodel"; first iSteps.
-    iStep --silent / as (Hsuffix%suffix_fmap) "Hmodel"; last congruence.
-    iDestruct (big_sepL2_snoc_2 with "Hslots_vs Hslot") as "#Hslots_vs'".
-    rewrite -fmap_snoc. iSteps.
-    iApply (big_sepL2_ref_pointsto_suffix with "Hslots_vs Hslots_ws"); first done.
+    awp_apply (base.inf_ws_deque_2_push_spec with "[$]").
+    { iApply (aacc_aupd_commit with "HΦ"); first done. iIntros "%vs (:model =1)". simplify.
+      iDestruct (meta_agree with "Hmeta_1 Hmeta_2") as %<-. iClear "Hmeta_2".
+      iAaccIntro with "Hmodel_1"; iSteps.
+    }
   Qed.
 
   Lemma inf_ws_deque_2_steal_spec t ι :
@@ -228,20 +679,13 @@ Section inf_ws_deque_2_G.
       True
     >>>.
   Proof.
-    iIntros "%Φ #Hinv HΦ".
+    iIntros "%Φ (:inv) HΦ".
 
-    wp_rec.
-
-    awp_smart_apply (inf_ws_deque_1_steal_spec with "Hinv").
-    iApply (aacc_aupd_commit with "HΦ"); first done. iIntros "%vs (:model)".
-    iAaccIntro with "Hmodel"; first iSteps.
-    iStep as "Hmodel".
-    destruct slots_vs as [| slot slots_vs], vs as [| v vs] => //.
-
-    - iFrame "#". iSteps.
-
-    - iDestruct "Hslots_vs" as "/= (Hslot & Hslots_vs)".
-      iSteps.
+    awp_apply (base.inf_ws_deque_2_steal_spec with "[$]").
+    { iApply (aacc_aupd_commit with "HΦ"); first done. iIntros "%vs (:model =1)". simplify.
+      iDestruct (meta_agree with "Hmeta Hmeta_1") as %->. iClear "Hmeta".
+      iAaccIntro with "Hmodel_1"; iSteps.
+    }
   Qed.
 
   Lemma inf_ws_deque_2_pop_spec t ι ws :
@@ -270,31 +714,19 @@ Section inf_ws_deque_2_G.
       inf_ws_deque_2_owner t ws'
     >>>.
   Proof.
-    iIntros "%Φ (#Hinv & (:owner)) HΦ".
+    iIntros "%Φ ((:inv =1) & (:owner =2)) HΦ". simplify.
+    iDestruct (meta_agree with "Hmeta_1 Hmeta_2") as %->. iClear "Hmeta_1".
 
-    wp_rec.
-
-    awp_smart_apply (inf_ws_deque_1_pop_spec with "[$Hinv $Howner]").
-    iApply (aacc_aupd_commit with "HΦ"); first done. iIntros "%vs (:model)".
-    iAaccIntro with "Hmodel"; first iSteps.
-    iStep 3 --silent / as (o slots_ws' Hsuffix%suffix_fmap) "Ho"; last congruence.
-    iDestruct (big_sepL2_ref_pointsto_suffix with "Hslots_vs Hslots_ws") as %?; first done.
-    destruct o as [𝑠𝑙𝑜𝑡 |].
-
-    - iDestruct "Ho" as "(%𝑠𝑙𝑜𝑡s & %Hslots & -> & Hmodel)".
-      apply fmap_snoc_inv in Hslots as (slots' & slot & -> & -> & ->).
-      iDestruct (big_sepL2_snoc_inv_l with "Hslots_vs") as "(%vs' & %v & -> & #Hslots' & #Hslot)".
-      iExists (Some v). iFrameSteps.
-
-    - iDestruct "Ho" as "(%Hslots & -> & Hmodel)".
-      apply fmap_nil_inv in Hslots as ->.
-      iDestruct (big_sepL2_nil_inv_l with "Hslots_vs") as %->.
-      iExists None. iSteps. do 2 (iExists []; iSteps).
+    awp_apply (base.inf_ws_deque_2_pop_spec with "[$]").
+    { iApply (aacc_aupd_commit with "HΦ"); first done. iIntros "%vs (:model =1)". simplify.
+      iDestruct (meta_agree with "Hmeta_1 Hmeta_2") as %<-. iClear "Hmeta_2".
+      iAaccIntro with "Hmodel_1". 1: iSteps. iIntros "%o %ws' ($ & Ho)".
+      iExists o, ws'. destruct o.
+      all: iDecompose "Ho".
+      all: iFrameSteps.
+    }
   Qed.
 End inf_ws_deque_2_G.
-
-From zoo_saturn Require
-  inf_ws_deque_2__opaque.
 
 #[global] Opaque inf_ws_deque_2_inv.
 #[global] Opaque inf_ws_deque_2_model.
